Auto/Embedding/LamTermInterp.lean
@@ -1,0 +1,7 @@
+import Auto.Embedding.LamBase
+
+namespace Auto.Embedding.Lam
+
+
+
+end Auto.Embedding.Lam
